\subsection*{Convergence of Holden Raynaud}
Helge Holden and Xavier Raynaud proved the convergence of their finite difference scheme in their article, under the assumption that $u_{0} - u_{0}'' \geq 0$ for initial data $u_{0} \in H^{1}([0,1])$. This proof is far beyond the scope of our course, so only an outline of the proof will be provided. \\

First, it is shown that if $m_{i}(0) \geq 0 \; \forall \;i$, then any solution $u(t)$ will have $m_{i}(t) \geq 0 \; \forall \;i $. Further, a uniform bound on the $H^{1}$ norm of the sequence $u^{n}$ in [0,T] is established. This also guarantees the existence of solutions in [0,T] for any given $T > 0$, since $\text{max}_{i}|u_{i}^{n}(t)| = \|u^{n}(\cdot,t)\|_{L^{\infty}} \leq \mathcal{O}(1) \|u^{n}\|_{H^{1}}$ remains bounded.

After this, it is shown that $u_{x}^{n}$ and $u_{t}^{n}$ are bounded in $L^{2}([0,1])$, and that $u_{x}^{n}$ has a uniformly bounded total variation. This is enough to prove that one can extract a converging subsequence of $u^{n}$, and that the limit is a solution of the Camassa-Holm equation. 

\subsection*{Consistency}
Our scheme is as following:
\begin{align}
m &= u - D_- D_+ u \\
m_t &=- D_- ( m u ) - m D ( u ),
\end{align}
where the operators are defined as

\begin{align}
D_- D_+ \left( U_j^n \right)  &= \frac{U_{j-1}^n - 2 U_j^n + U_{j+1}^n}{h^2} = \frac{\partial}{\partial x} (u) + O \left( h^ 2 \right) \\
 D_- \left(M_j^n U_j^n \right) &= U_j^n D_-( M_j^n ) + M_j^n D_- (U_j^n) \\
  &= M_j^n \frac{U_J^n - U_{j-1}^n}{h} + U_j^n \frac{M_{j}^n - M_{j-1}^n}{h} \\
  &= m \frac{\partial}{\partial x} (u) + u \frac{\partial}{\partial x} (m) + O \left( h \right)  \\
D \left(U_j^n \right) &= \frac{U_{j+1}^n - U_{j-1}^n}{2h} = \frac{\partial}{\partial x} (u) + O \left( h \right).
\end{align}

If we also use forward Euler to integrate we get that
\begin{align}
D_+ (m) = \frac{M_j^{n+1} - M_j^n}{k} =  \frac{\partial}{\partial t} (m) + O(k^2).
\end{align}

Putting this back into the equation we get that

\begin{align}
m &= u - \left( u_{xx} + O\left(h^2\right) \right) \\
m_t  + O(k^2) &= - \left( m u_x + u m_x + O(h) \right) - m \left( u_x + O(h) \right)
\end{align}

Letting the timestep and spacestep go to zero, we get
\begin{align}
m &= u - u_{xx} \\
m_t &= - m u_x - u m_x - m u_x = - 2m u_x - u m_x
\end{align}
which is exactly the Camassa-Holm equation that we're trying to solve. Our scheme is consistent.